Sections, explicit type X, some proof slightly shorter

Front.v
@@ -7,26 +7,30 @@ From CritBit Require Import KeyUtil.
 From CritBit Require Import PrefixCritical.
 From CritBit Require Import SeqAccess.
 
+Section Critbit.
+
+Context (X : Type).
+
 (* a CBT (non-empty) *)
-Inductive CBT {X : Type} : Type :=
+Inductive CBT : Type :=
   | Leaf (k : list bool) (v : X)
   | Branch (i : nat) (l r : CBT).
 
 (* precond: one-terminated k *)
 (* precond: t is a valid tree w.r.t. CBT_valid *)
-Fixpoint lookup {X : Type} (k : list bool) (t : CBT) : option X :=
+Fixpoint lookup (k : list bool) (t : CBT) : option X :=
   match t with
   | Leaf k' v => if key_eqb k k' then Some v else None
   | Branch i l r => if ith_zer i k then lookup k r else lookup k l
   end.
 
-Fixpoint find_best_key {X : Type} (k : list bool) (t : @CBT X) : (list bool) :=
+Fixpoint find_best_key (k : list bool) (t : CBT) : (list bool) :=
   match t with
   | Leaf k' _ => k'
   | Branch i l r => find_best_key k (if ith_zer i k then r else l)
   end.
 
-Definition seed {X : Type} (k : list bool) (v : X) : CBT :=
+Definition seed (k : list bool) (v : X) : CBT :=
   Leaf k v.
 
 Definition is_beforeb (pos : option nat) (bound : nat) : bool :=
@@ -35,12 +39,12 @@ Definition is_beforeb (pos : option nat) (bound : nat) : bool :=
   | Some i => i <? bound
   end.
 
-Definition insert_as_branch {X : Type} (k : list bool) (v : X) (i : nat) (t : CBT) : CBT :=
+Definition insert_as_branch (k : list bool) (v : X) (i : nat) (t : CBT) : CBT :=
   if ith_zer i k then Branch i t (Leaf k v) else Branch i (Leaf k v) t.
 
 (* precond: t is a valid tree w.r.t. CBT_valid *)
 (* precond: i is the critical bit of k w.r.t. t *)
-Fixpoint insert_at {X : Type} (k : list bool) (v : X) (i : option nat) (t : CBT) : CBT :=
+Fixpoint insert_at (k : list bool) (v : X) (i : option nat) (t : CBT) : CBT :=
   match t with
   | Leaf k' v' =>  match i with
                    | None => Leaf k v
@@ -56,9 +60,11 @@ Fixpoint insert_at {X : Type} (k : list bool) (v : X) (i : option nat) (t : CBT)
             else Branch j (insert_at k v i l) r)
   end.
 
-Definition critical_bit_CBT {X : Type} (k : list bool) (t : @CBT X) : option nat :=
+Definition critical_bit_CBT (k : list bool) (t : CBT) : option nat :=
   critical_bit_zer k (find_best_key k t).
 
 (* precond: one-terminated k *)
-Definition insert {X : Type} (k : list bool) (v : X) (t : CBT) : CBT :=
+Definition insert (k : list bool) (v : X) (t : CBT) : CBT :=
   insert_at k v (critical_bit_CBT k t) t.
+
+End Critbit.
