Main.v
@@ -20,6 +20,7 @@ Require Import Bool.
 Require Import Arith.
 Require Import Arith.Compare.
 Require Import Logic.FunctionalExtensionality.
+Require Import Lia.
 Import ListNotations.
 
 From CritBit Require Import Front.
@@ -28,53 +29,54 @@ From CritBit Require Import KeyUtil.
 From CritBit Require Import PrefixCritical.
 From CritBit Require Import SeqAccess.
 
-Definition content_map (X : Type) : Type := list bool -> option X.
+Section Critbit.
 
-Definition singleton {X : Type} (k : list bool) (v : X) : content_map X
+  Context (X : Type).
+
+Definition content_map : Type := list bool -> option X.
+
+Definition singleton (k : list bool) (v : X) : content_map
   := fun k' => if key_eqb k k' then Some v else None.
 
-Definition cbit_union {X : Type} (cbit : nat) (m0 m1 : content_map X) : content_map X
+Definition cbit_union (cbit : nat) (m0 m1 : content_map) : content_map
   := fun k' => if ith_zer cbit k' then m1 k' else m0 k'.
 
-Inductive pmCBT_valid {X : Type} : prefix -> content_map X -> @CBT X -> Prop :=
+Inductive pmCBT_valid : prefix -> content_map -> CBT X -> Prop :=
 | pcv_leaf (k : list bool) (v : X) (H : OneTerminated k)
-  : pmCBT_valid (ZeroExt k) (singleton k v) (Leaf k v)
-| pcv_branch (p : list bool) (pl pr : prefix) (ml mr : content_map X) (l r : CBT)
+  : pmCBT_valid (ZeroExt k) (singleton k v) (Leaf X k v)
+| pcv_branch (p : list bool) (pl pr : prefix) (ml mr : content_map) (l r : CBT X)
     (Hl : pmCBT_valid pl ml l) (Hr : pmCBT_valid pr mr r)
     (Hpl : is_prefix (p ++ [false]) pl) (Hpr : is_prefix (p ++ [true]) pr)
-  : pmCBT_valid (Finite p) (cbit_union (length p) ml mr) (Branch (length p) l r).
+  : pmCBT_valid (Finite p) (cbit_union (length p) ml mr) (Branch X (length p) l r).
 
-Definition pCBT_valid {X : Type} (p : prefix) (t : @CBT X) : Prop :=
+Definition pCBT_valid (p : prefix) (t : CBT X) : Prop :=
   exists m, pmCBT_valid p m t.
 
-Lemma pmCBT_valid_forget_m : forall (X : Type)
-                                    (p : prefix) (m : content_map X) (t : CBT),
+Lemma pmCBT_valid_forget_m : forall (p : prefix) (m : content_map) (t : CBT X),
     pmCBT_valid p m t -> pCBT_valid p t.
 Proof.
-  intros X p m t H. exists m. assumption.
+  intros. eexists. eassumption.
 Qed.
 
-Definition mCBT_valid {X : Type} (m : content_map X) (t : @CBT X) : Prop :=
+Definition mCBT_valid (m : content_map) (t : CBT X) : Prop :=
   exists p, pmCBT_valid p m t.
 
-Lemma pmCBT_valid_forget_p : forall (X : Type)
-                                    (p : prefix) (m : content_map X) (t : CBT),
+Lemma pmCBT_valid_forget_p : forall (p : prefix) (m : content_map) (t : CBT X),
     pmCBT_valid p m t -> mCBT_valid m t.
 Proof.
-  intros. exists p. assumption.
+  intros. eexists. eassumption.
 Qed.
 
-Definition CBT_valid {X : Type} (t : @CBT X) : Prop :=
+Definition CBT_valid (t : @CBT X) : Prop :=
   exists p m, pmCBT_valid p m t.
 
 (* ROOM FOR IMPROVEMENT: prove this lemma using the one one below and
    a lemma that the best key is in the content map *)
-Lemma best_key_has_prefix : forall (X : Type) (k p : list bool)
-                                   (t : @CBT X),
+Lemma best_key_has_prefix : forall (k p : list bool) (t : @CBT X),
     pCBT_valid (Finite p) t ->
-    is_prefix_zer p (find_best_key k t).
+    is_prefix_zer p (find_best_key X k t).
 Proof.
-  intros X k p t. generalize dependent p. induction t.
+  intros k p t. generalize dependent p. induction t.
   - intros p H. destruct H. inversion H.
   - intros p H. simpl. destruct H as [m H]. inversion H. rewrite <- H3 in H.
     clear l r H3 H4 H5 p0 H1 i H0.
@@ -91,8 +93,7 @@ Proof.
         apply (prefix_zer_trans p p0 _ Hpl IHt1).
 Qed.
 
-Lemma key_has_prefix : forall (X : Type) (k p : list bool) (m : content_map X)
-                                (t : CBT),
+Lemma key_has_prefix : forall (k p : list bool) (m : content_map) (t : CBT X),
     pmCBT_valid (Finite p) m t -> (exists v, m k = Some v) -> is_prefix_zer p k.
 Proof.
   intros. remember (Finite p) as pi. generalize dependent p.
@@ -116,24 +117,23 @@ Proof.
         eapply prefix_zer_trans. eassumption. assumption.
 Qed.
 
-Lemma best_key_one_terminated : forall (X : Type) (k : list bool) (t : @CBT X),
-    CBT_valid t -> OneTerminated (find_best_key k t).
+Lemma best_key_one_terminated : forall (k : list bool) (t : @CBT X),
+    CBT_valid t -> OneTerminated (find_best_key X k t).
 Proof.
   induction t.
   - intro H. unfold CBT_valid in H. destruct H as [m [p H]]. inversion H. simpl.
     assumption.
-  - intro H. simpl. unfold CBT_valid in *. destruct H as [m [p0 H]]. inversion H. rewrite <- H3 in *.
-    destruct (ith_zer (length p) k).
-    + apply IHt2. exists pr. exists mr. assumption.
-    + apply IHt1. exists pl. exists ml. assumption.
+  - intro H. simpl. unfold CBT_valid in *. destruct H as [m [p0 H]]. inversion H.
+    subst. 
+    destruct (ith_zer (length p) k); try eapply IHt1; try eapply IHt2;
+      eexists; eexists; eassumption.
 Qed.
 
 Lemma is_beforeb_true_exists : forall (o : option nat) (m : nat),
     is_beforeb o m = true -> exists n, o = Some n /\ S n <= m.
 Proof.
   intros o m H. destruct o.
-  - simpl in H. exists n. split. reflexivity. apply Nat.ltb_lt in H.
-    unfold "<" in H. assumption.
+  - simpl in H. eexists. split. reflexivity. apply Nat.ltb_lt in H. lia.
   - discriminate.
 Qed.
 
@@ -141,99 +141,96 @@ Lemma is_beforeb_false_high_none : forall (o : option nat) (m : nat),
     is_beforeb o m = false -> (o = None \/ exists n, o = Some n /\ m <= n).
 Proof.
   intros o m H. destruct o.
-  - simpl in H. right. exists n. split. reflexivity. apply Nat.ltb_ge. assumption.
-  - left. reflexivity.
+  - simpl in H. right. eexists. split. reflexivity. apply Nat.ltb_ge. assumption.
+  - tauto.
 Qed.
 
-Lemma high_critbit_is_prefix : forall (X : Type) (k p : list bool) (t : @CBT X),
+Lemma high_critbit_is_prefix : forall (k p : list bool) (t : @CBT X),
     pCBT_valid (Finite p) t ->
-    is_beforeb (critical_bit_CBT k t) (length p) = false ->
+    is_beforeb (critical_bit_CBT X k t) (length p) = false ->
     is_prefix_zer p k.
 Proof.
-  intros X k p t H1 H2. destruct H1 as [m H1]. inversion H1. rewrite <- H4 in *.
-  clear t H4 p0 H0 H3. apply is_beforeb_false_high_none in H2.
+  intros k p t H1 H2. destruct H1 as [m H1]. inversion H1. subst.
+  apply is_beforeb_false_high_none in H2.
   apply pmCBT_valid_forget_m in H1. apply best_key_has_prefix with (k:=k) in H1.
   apply prefix_iff_take_eq in H1. unfold critical_bit_CBT in H2.
-  remember (find_best_key k (Branch (length p) l r)) as k'.
+  remember (find_best_key X k (Branch X (length p) l r)) as k'.
   assert (take_zer (length p) k = take_zer (length p) k').
   { destruct H2.
-    - rewrite critical_bit_zer_none_eqv in H. specialize (H (length p)). assumption.
+    - rewrite critical_bit_zer_none_eqv in H. auto.
     - destruct H as [n [H2 H3]]. apply critical_bit_zer_take_eq in H2.
-      rewrite <- (take_take _ n _). rewrite H2. rewrite take_take. reflexivity.
-      assumption. assumption. }
-  apply prefix_iff_take_eq. rewrite H. assumption.
+      erewrite <- take_take; [| eassumption]. rewrite H2.
+      rewrite take_take; [| assumption]. reflexivity. }
+  apply prefix_iff_take_eq. congruence. 
 Qed.
 
-Lemma low_critbit_on_prefix : forall (X : Type) (k p : list bool) (t : @CBT X),
+Lemma low_critbit_on_prefix : forall (k p : list bool) (t : @CBT X),
     pCBT_valid (Finite p) t ->
-    is_beforeb (critical_bit_CBT k t) (length p) = true ->
-    critical_bit_CBT k t = critical_bit_fin k p.
+    is_beforeb (critical_bit_CBT X k t) (length p) = true ->
+    critical_bit_CBT X k t = critical_bit_fin k p.
 Proof.
-  intros X k p t. generalize dependent p. induction t.
+  intros k p t. generalize dependent p. induction t.
   - intros p H. destruct H. inversion H.
   - intros p H1 H2. unfold critical_bit_CBT in *. simpl in *. destruct H1 as [m H1].
-    inversion H1. rewrite <- H in *. clear H5 l H6 r H0 p0 H i.
+    inversion H1. subst.
     apply app_is_prefix in Hpl. apply app_is_prefix in Hpr.
     assert (forall (ps : prefix) (t : @CBT X),
                (forall (p : list bool), pCBT_valid (Finite p) t ->
-                                      is_beforeb (critical_bit_zer k (find_best_key k t)) (length p) = true ->
-                                      critical_bit_zer k (find_best_key k t) = critical_bit_fin k p) ->
-               is_beforeb (critical_bit_zer k (find_best_key k t)) (length p) = true ->
+                                      is_beforeb (critical_bit_zer k (find_best_key X k t)) (length p) = true ->
+                                      critical_bit_zer k (find_best_key X k t) = critical_bit_fin k p) ->
+               is_beforeb (critical_bit_zer k (find_best_key X k t)) (length p) = true ->
                is_prefix p ps ->
                pCBT_valid ps t ->
-               critical_bit_zer k (find_best_key k t) = critical_bit_fin k p). {
+               critical_bit_zer k (find_best_key X k t) = critical_bit_fin k p). {
       clear. intros ps t H1 H2 H3 H4. apply is_beforeb_true_exists in H2.
       destruct H2 as [n [H5 H6]]. destruct ps.
-      - destruct H4 as [m H4]. inversion H4. rewrite <- H7 in *. clear H k0 H4 H7 t H2.
+      - destruct H4 as [m H4]. inversion H4. subst.
         simpl in *. rewrite H5.
         symmetry. apply critical_bit_zer_fin. assumption.
         apply prefix_iff_take_eq in H3. rewrite <- H3. apply critical_bit_zer_from_parts.
         apply critical_bit_zer_take_eq in H5. rewrite take_take.
-        assumption. apply Le.le_Sn_le_stt. assumption. rewrite ith_from_take.
+        assumption. lia. rewrite ith_from_take.
         apply critical_bit_zer_ith_neq in H5. assumption. assumption.
       - specialize (H1 p0 H4).
-        pose proof (best_key_has_prefix X k p0 t H4).
-        remember (find_best_key k t) as k'. clear Heqk' H4. simpl in H3.
+        pose proof (best_key_has_prefix k p0 t H4).
+        remember (find_best_key X k t) as k'. clear Heqk' H4. simpl in H3.
         rewrite H5 in *. clear H5. simpl in H1. rewrite Nat.ltb_lt in H1.
-        unfold "<" in H1. assert (S n <= length p0). transitivity (length p).
-        assumption. apply is_prefix_fin_length. assumption. specialize (H1 H0).
+        unfold "<" in H1. assert (S n <= length p0). apply is_prefix_fin_length in H3.
+        lia. specialize (H1 H0).
         symmetry. symmetry in H1. apply critical_bit_fin_zer in H1.
         apply critical_bit_zer_fin. assumption. apply is_prefix_fin_zer in H3.
         apply prefix_iff_take_eq in H3. rewrite <- H3.
         apply critical_bit_zer_from_parts. rewrite take_take.
-        apply critical_bit_zer_take_eq in H1. assumption. apply Le.le_Sn_le_stt.
-        assumption. rewrite ith_from_take. apply critical_bit_zer_ith_neq in H1.
+        apply critical_bit_zer_take_eq in H1. assumption. lia.
+        rewrite ith_from_take. apply critical_bit_zer_ith_neq in H1.
         assumption. assumption.
     } destruct (ith_zer (length p) k).
-    + apply pmCBT_valid_forget_m in Hr. apply (H pr t2 IHt2 H2 Hpr Hr).
+    + apply pmCBT_valid_forget_m in Hr. eapply H; eassumption.
     + apply pmCBT_valid_forget_m in Hl. apply (H pl t1 IHt1 H2 Hpl Hl).
 Qed.
 
-Lemma pcv_finite_len_num : forall (X : Type) (p : list bool) (plen : nat)
-                                  (pl pr : prefix) (l r : CBT),
+Lemma pcv_finite_len_num : forall (p : list bool) (plen : nat)
+                                  (pl pr : prefix) (l r : CBT X),
     length p = plen -> is_prefix (p ++ [false]) pl -> is_prefix (p ++ [true]) pr ->
-    pCBT_valid pl l -> pCBT_valid pr r -> @pCBT_valid X (Finite p) (Branch plen l r).
+    pCBT_valid pl l -> pCBT_valid pr r -> @pCBT_valid (Finite p) (Branch X plen l r).
 Proof.
-  intros *. intros H1 H2 H3 H4 H5. rewrite <- H1.
-  destruct H4 as [ml H4]. destruct H5 as [mr H5].
-  exists (fun k' => if ith_zer (length p) k' then mr k' else ml k').
-  apply pcv_branch with (pl:=pl) (pr:=pr).
-  assumption. assumption. assumption. assumption.
+  intros. subst. destruct H2. destruct H3. 
+  eexists. econstructor; eassumption.
 Qed.
 
-Lemma pmcv_finite_len_num : forall (X : Type) (p : list bool) (plen : nat)
-                                   (pl pr : prefix) (ml mr : content_map X) (l r : CBT),
+Lemma pmcv_finite_len_num : forall (p : list bool) (plen : nat)
+                                   (pl pr : prefix) (ml mr : content_map) (l r : CBT X),
     length p = plen -> is_prefix (p ++ [false]) pl -> is_prefix (p ++ [true]) pr ->
     pmCBT_valid pl ml l -> pmCBT_valid pr mr r ->
-    pmCBT_valid (Finite p) (cbit_union plen ml mr) (Branch plen l r).
+    pmCBT_valid (Finite p) (cbit_union plen ml mr) (Branch X plen l r).
 Proof.
   intros. rewrite <- H. econstructor; eassumption.
 Qed.
 
-Definition cmap_insert {X : Type} (k : list bool) (v : X) (m : content_map X)
-  : content_map X := (fun k' => if key_eqb k k' then Some v else m k').
+Definition cmap_insert (k : list bool) (v : X) (m : content_map)
+  : content_map := (fun k' => if key_eqb k k' then Some v else m k').
 
-Lemma cmap_insert_cbit_singleton : forall (X : Type) (k0 k : list bool) (v0 v : X)
+Lemma cmap_insert_cbit_singleton : forall (k0 k : list bool) (v0 v : X)
                                           (n : nat),
     critical_bit_zer k k0 = Some n ->
     cmap_insert k v (singleton k0 v0) = if ith_zer n k then
@@ -241,29 +238,29 @@ Lemma cmap_insert_cbit_singleton : forall (X : Type) (k0 k : list bool) (v0 v : 
                                         else
                                           cbit_union n (singleton k v) (singleton k0 v0).
 Proof.
-  intros X k0 k v0 v n H1. unfold cmap_insert. unfold cbit_union.
-  apply critical_bit_zer_ith_neq in H1. extensionality k''. unfold singleton.
+  intros. unfold cmap_insert. unfold cbit_union.
+  apply critical_bit_zer_ith_neq in H. extensionality k''. unfold singleton.
   destruct (key_eqb k k'') eqn:E.
   - apply key_eqb_iff in E. subst k''.
-    destruct (ith_zer n k) eqn:E2; apply not_eq_sym in H1; rewrite E2;
-    rewrite (key_eqb_reflx k); reflexivity.
-  - destruct (ith_zer n k) eqn:E2; apply bneq_eq_neg in H1; symmetry in H1; simpl in H1;
-    rewrite E; destruct (key_eqb k0 k'') eqn:E3; try (apply key_eqb_iff in E3; subst;
-    rewrite H1; reflexivity); destruct (ith_zer n k''); reflexivity.
+    destruct (ith_zer n k) eqn:E2; apply not_eq_sym in H; rewrite E2;
+    rewrite key_eqb_reflx; reflexivity.
+  - destruct (ith_zer n k) eqn:E2; apply bneq_eq_neg in H; simpl in H; rewrite E;
+    destruct (key_eqb k0 k'') eqn:E3; try (apply key_eqb_iff in E3; subst;
+    rewrite <- H; reflexivity); destruct (ith_zer n k''); reflexivity.
 Qed.
 
-Lemma cmap_insert_eqk_singleton : forall (X : Type) (k : list bool) (v0 v : X),
+Lemma cmap_insert_eqk_singleton : forall (k : list bool) (v0 v : X),
   cmap_insert k v (singleton k v0) = singleton k v.
 Proof.
   intros. extensionality k'. unfold cmap_insert. unfold singleton.
   destruct (key_eqb k k'); reflexivity.
 Qed.
 
-Lemma cmap_insert_low_cb_branch : forall (X : Type) (k : list bool) (v : X)
-                                         (p : list bool) (m : content_map X)
+Lemma cmap_insert_low_cb_branch : forall (k : list bool) (v : X)
+                                         (p : list bool) (m : content_map)
                                          (l r : @CBT X) (n : nat),
-    pmCBT_valid (Finite p) m (Branch (length p) l r) ->
-    critical_bit_CBT k (Branch (length p) l r) = Some n -> n < length p ->
+    pmCBT_valid (Finite p) m (Branch X (length p) l r) ->
+    critical_bit_CBT X k (Branch X (length p) l r) = Some n -> n < length p ->
     cmap_insert k v m = if ith_zer n k then
                           cbit_union n m (singleton k v)
                         else
@@ -289,11 +286,11 @@ Proof.
         destruct (ith_zer n k0); reflexivity.
 Qed.
 
-Lemma cmap_insert_high_cb_branch : forall (X : Type) (k : list bool) (v : X)
-                                          (p : list bool) (ml mr : content_map X)
+Lemma cmap_insert_high_cb_branch : forall (k : list bool) (v : X)
+                                          (p : list bool) (ml mr : content_map)
                                           (l r : @CBT X),
-    pmCBT_valid (Finite p) (cbit_union (length p) ml mr) (Branch (length p) l r) ->
-    is_beforeb (critical_bit_CBT k (Branch (length p) l r)) (length p) = false ->
+    pmCBT_valid (Finite p) (cbit_union (length p) ml mr) (Branch X (length p) l r) ->
+    is_beforeb (critical_bit_CBT X k (Branch X (length p) l r)) (length p) = false ->
     cmap_insert k v (cbit_union (length p) ml mr)
     = if ith_zer (length p) k then
         cbit_union (length p) ml (cmap_insert k v mr)
@@ -307,11 +304,11 @@ Proof.
     try (apply key_eqb_iff in E; subst k0); try rewrite E2; try reflexivity.
 Qed.
 
-Theorem insert_correct {X : Type} :
-  forall (p : prefix) (m : content_map X) (t : CBT) (k : list bool) (v : X)
+Theorem insert_correct :
+  forall (p : prefix) (m : content_map) (t : CBT X) (k : list bool) (v : X)
          (p' : list bool),
     pmCBT_valid p m t -> is_prefix p' p -> is_prefix_zer p' k -> OneTerminated k ->
-    exists pi, is_prefix p' pi /\ pmCBT_valid pi (cmap_insert k v m) (insert k v t).
+    exists pi, is_prefix p' pi /\ pmCBT_valid pi (cmap_insert k v m) (insert X k v t).
 Proof.
   intros p m t k v p' H. generalize dependent p'. induction H.
   - intros p' H1 H2 H3. unfold insert. unfold critical_bit_CBT. simpl.
@@ -327,9 +324,9 @@ Proof.
       * unfold insert_as_branch. pose proof (critical_bit_zer_ith_neq _ _ _ E).
         pose proof E as Hcb.
         apply critical_bit_zer_prefix in E.
-        assert (pmCBT_valid (ZeroExt k0) (singleton k0 v0) (Leaf k0 v0)).
+        assert (pmCBT_valid (ZeroExt k0) (singleton k0 v0) (Leaf X k0 v0)).
         { constructor. assumption. }
-        assert (pmCBT_valid (ZeroExt k) (singleton k v) (Leaf k v)).
+        assert (pmCBT_valid (ZeroExt k) (singleton k v) (Leaf X k v)).
         { apply pcv_leaf. assumption. }
         assert (is_prefix (take_zer n k ++ [negb (ith_zer n k)]) (ZeroExt k0)).
         { simpl. assumption. }
@@ -341,16 +338,13 @@ Proof.
         -- destruct (ith_zer n k); rewrite <- (take_length n k) at 2;
            rewrite <- (take_length n k) at 3; econstructor; eassumption.
         -- assumption.
-    + exists (ZeroExt k). apply (critical_bit_zer_none_eq k k0) in E. subst k0. split.
-      * assumption.
-      * rewrite cmap_insert_eqk_singleton. constructor. assumption.
-      * assumption.
-      * assumption.
+    + eexists. apply critical_bit_zer_none_eq in E; try assumption. split.
+      * eassumption.
+        * subst k. rewrite cmap_insert_eqk_singleton. constructor. assumption.
   - intros p' H1 H2 H3. unfold insert. simpl. 
-    destruct ((is_beforeb (critical_bit_CBT k (Branch (length p) l r))) (length p)) eqn:E.
-    + pose proof (low_critbit_on_prefix X k p (Branch (length p) l r)).
-      Print pcv_branch.
-      specialize (H4 (pmCBT_valid_forget_m _ _ _ _ (pcv_branch p pl pr ml mr l r H H0 Hpl Hpr)) E). rewrite H4 in *. apply is_beforeb_true_exists in E. destruct E as [n [H5 H6]].
+    destruct ((is_beforeb (critical_bit_CBT X k (Branch X (length p) l r))) (length p)) eqn:E.
+    + pose proof (low_critbit_on_prefix k p (Branch X (length p) l r)).
+      specialize (H4 (pmCBT_valid_forget_m _ _ _ (pcv_branch p pl pr ml mr l r H H0 Hpl Hpr)) E). rewrite H4 in *. apply is_beforeb_true_exists in E. destruct E as [n [H5 H6]].
       rewrite H5. exists (Finite (take_zer n p)). split.
       * simpl. simpl in H1. assert (length p' <= n).
         destruct (le_le_S_dec (length p') n).
@@ -359,21 +353,20 @@ Proof.
         apply is_prefix_fin_zer in H1. apply prefix_iff_take_eq in H1.
         assert (ith_zer n p' = ith_zer n p'). reflexivity. rewrite <- H1 in H7 at 2.
         rewrite <- H2 in H7 at 1. rewrite ith_from_take in H7.
-        rewrite ith_from_take in H7. apply H5 in H7. destruct H7. assumption.
+        rewrite ith_from_take in H7. contradiction. assumption.
         assumption. apply is_prefix_zer_fin. split. apply prefix_iff_take_eq.
         apply is_prefix_fin_zer in H1. apply prefix_iff_take_eq in H1.
         rewrite take_take. assumption. assumption. rewrite take_length. assumption.
       * unfold insert_as_branch.
         assert (take_zer n k = take_zer n p).
-        { apply critical_bit_fin_zer in H5. apply (critical_bit_zer_take_eq _ _ _ H5). }
+        { apply critical_bit_fin_zer in H5. apply critical_bit_zer_take_eq. assumption. }
         assert (is_prefix (take_zer n p ++ [negb (ith_zer n k)]) (Finite p)).
         { simpl. pose proof (critical_bit_fin_prefix _ _ _ H5).          
           rewrite H7 in H8. assumption. }
         assert (is_prefix (take_zer n p ++ [ith_zer n k]) (ZeroExt k)).
         { simpl. rewrite <- H7. rewrite take_with_ith. apply take_is_prefix. }
-        Print pcv_branch.
         assert (pmCBT_valid (Finite p) (cbit_union (length p) ml mr)
-                  (Branch (length p) l r)).
+                  (Branch X (length p) l r)).
         { eapply pcv_branch; eassumption. }
         destruct (ith_zer n k) eqn:E; erewrite cmap_insert_low_cb_branch;
           try erewrite E; try eapply pmcv_finite_len_num; try apply take_length;
@@ -391,11 +384,13 @@ Proof.
         try eassumption.
 Qed.
 
-Theorem lookup_correct : forall (X : Type) (p : prefix) (m : content_map X) (t : CBT)
+Theorem lookup_correct : forall (p : prefix) (m : content_map) (t : CBT X)
                                 (k : list bool),
-    OneTerminated k -> pmCBT_valid p m t -> lookup k t = m k.
+    OneTerminated k -> pmCBT_valid p m t -> lookup X k t = m k.
 Proof.
   intros. induction H0.
   - unfold singleton. rewrite key_eqb_sym. reflexivity.
   - unfold cbit_union. simpl. destruct (ith_zer (length p) k); assumption.
 Qed.
+
+End Critbit.
